veric/binop_lemmas.v
@@ -1,7 +1,6 @@
-Require Import VST.msl.msl_standard.
 Require Import VST.veric.Clight_base.
-Require Import VST.veric.compcert_rmaps.
 Require Import VST.veric.Clight_lemmas.
+Require Import VST.veric.res_predicates.
 Require Import VST.veric.mpred.
 Require Import VST.veric.tycontext.
 Require Import VST.veric.expr2.
@@ -13,13 +12,17 @@ Require Import VST.veric.binop_lemmas5.
 Require Import VST.veric.binop_lemmas6.
 Import Cop.
 
+Section mpred.
+
+Context `{!heapGS Σ}.
+
 Lemma typecheck_binop_sound:
-forall op {CS: compspecs} (rho : environ) m (e1 e2 : expr) (t : type)
-   (IBR: denote_tc_assert (isBinOpResultType op e1 e2 t) rho m)
+forall op {CS: compspecs} (rho : environ) (e1 e2 : expr) (t : type)
    (TV2: tc_val (typeof e2) (eval_expr e2 rho))
    (TV1: tc_val (typeof e1) (eval_expr e1 rho)),
-   tc_val t
-     (eval_binop op (typeof e1) (typeof e2) (eval_expr e1 rho) (eval_expr e2 rho)).
+   denote_tc_assert (isBinOpResultType op e1 e2 t) rho ⊢
+   ⌜tc_val t
+     (eval_binop op (typeof e1) (typeof e2) (eval_expr e1 rho) (eval_expr e2 rho))⌝.
 Proof.
   intros.
   destruct op;
@@ -35,3 +38,4 @@ Proof.
     | eapply typecheck_Otest_order_sound; solve [eauto]].
 Qed.
 
+End mpred.
