veric/binop_lemmas5.v
@@ -1,7 +1,6 @@
-Require Import VST.msl.msl_standard.
 Require Import VST.veric.Clight_base.
-Require Import VST.veric.compcert_rmaps.
 Require Import VST.veric.Clight_lemmas.
+Require Import VST.veric.res_predicates.
 Require Import VST.veric.mpred.
 Require Import VST.veric.tycontext.
 Require Import VST.veric.expr2.
@@ -12,20 +11,24 @@ Import Cop.
 
 Transparent intsize_eq.
 
+Section mpred.
+
+Context `{!heapGS Σ}.
+
+(*Lemma test: ∀ (cmp : comparison) (v1 v2 v : val)
+    sem_cmp_pp cmp v1 v2 = Some v*)
+
 Lemma typecheck_Otest_eq_sound:
- forall op {CS: compspecs} (rho : environ) m (e1 e2 : expr) (t : type)
-   (IBR: denote_tc_assert (isBinOpResultType op e1 e2 t) rho m)
+ forall op {CS: compspecs} (rho : environ) (e1 e2 : expr) (t : type)
    (TV2: tc_val (typeof e2) (eval_expr e2 rho))
    (TV1: tc_val (typeof e1) (eval_expr e1 rho))
    (OP: op = Oeq \/ op = One),
-   tc_val t
-     (eval_binop op (typeof e1) (typeof e2) (eval_expr e1 rho) (eval_expr e2 rho)).
+   denote_tc_assert (isBinOpResultType op e1 e2 t) rho ⊢
+   ⌜tc_val t
+     (eval_binop op (typeof e1) (typeof e2) (eval_expr e1 rho) (eval_expr e2 rho))⌝.
 Proof.
   intros.
-  replace
-    ((denote_tc_assert (isBinOpResultType op e1 e2 t) rho) m)
-  with
-    ((denote_tc_assert
+  trans (denote_tc_assert
            match classify_cmp' (typeof e1) (typeof e2) with
               | Cop.cmp_default =>
                            tc_bool (is_numeric_type (typeof e1)
@@ -48,9 +51,8 @@ Proof.
               | Cop.cmp_case_lp => 
                      tc_andp' (tc_int_or_ptr_type (typeof e2))
                     (check_pp_int' (Ecast e1 size_t) e2 op t (Ebinop op e1 e2 t))
-           end rho) m)
-  in IBR
-  by (rewrite den_isBinOpR; destruct OP as [|]; subst; auto).
+           end rho);
+  first by (rewrite den_isBinOpR; destruct OP as [|]; subst; auto).
   replace
     (tc_val t (eval_binop op (typeof e1) (typeof e2) (eval_expr e1 rho) (eval_expr e2 rho)))
   with
@@ -76,63 +78,49 @@ Proof.
          | cmp_default => sem_cmp_default (op_to_cmp op) (typeof e1) (typeof e2)
          end (eval_expr e1 rho) (eval_expr e2 rho))))
   by (destruct OP as [|]; subst; rewrite <- classify_cmp_eq; auto).
-  unfold tc_int_or_ptr_type, eval_binop, sem_binary_operation', isBinOpResultType, Clight_Cop2.sem_add in IBR |- *.
+  unfold tc_int_or_ptr_type, eval_binop, sem_binary_operation', isBinOpResultType, Clight_Cop2.sem_add.
   unfold force_val;
-  rewrite tc_val_tc_val_PM in TV1,TV2.
+  rewrite !tc_val_tc_val_PM' in TV1,TV2.
   replace (check_pp_int' e1 e2 op t (Ebinop op e1 e2 t))
     with (tc_andp' (tc_test_eq' e1 e2)
                    (tc_bool (is_int_type t) (op_result_type (Ebinop op e1 e2 t))))
-    in IBR
     by (unfold check_pp_int'; destruct OP; subst; auto).
-  replace (check_pp_int' e1 (Ecast e2 (Tint I32 Unsigned noattr)) op t (Ebinop op e1 e2 t))
-    with (tc_andp' (tc_test_eq' e1 (Ecast e2 (Tint I32 Unsigned noattr)))
+  replace (check_pp_int' e1 (Ecast e2 size_t) op t (Ebinop op e1 e2 t))
+    with (tc_andp' (tc_test_eq' e1 (Ecast e2 size_t))
                    (tc_bool (is_int_type t) (op_result_type (Ebinop op e1 e2 t))))
-    in IBR
     by (unfold check_pp_int'; destruct OP; subst; auto).
-  replace (check_pp_int' (Ecast e1 (Tint I32 Unsigned noattr)) e2 op t (Ebinop op e1 e2 t))
-    with (tc_andp' (tc_test_eq' (Ecast e1 (Tint I32 Unsigned noattr)) e2)
+  replace (check_pp_int' (Ecast e1 size_t) e2 op t (Ebinop op e1 e2 t))
+    with (tc_andp' (tc_test_eq' (Ecast e1 size_t) e2)
                    (tc_bool (is_int_type t) (op_result_type (Ebinop op e1 e2 t))))
-    in IBR
     by (unfold check_pp_int'; destruct OP; subst; auto).
-Time (* 71 sec *)
-  destruct Archi.ptr64 eqn:Hp;
-  destruct (classify_cmp' (typeof e1) (typeof e2)) eqn:?H; try solve [inv IBR];
-try abstract (
-  destruct OP; subst op;
+  destruct Archi.ptr64 eqn:Hp; try discriminate;
+  pose proof (classify_cmp_reflect (typeof e1) (typeof e2)) as Hcmp; inv Hcmp; simpl; unfold_lift;
+    rewrite !tc_bool_e;
+  last (by rewrite -!tc_val_tc_val_PM' in TV1,TV2; rewrite !andb_true_iff; iPureIntro; intros ((? & ?) & ?); apply tc_val_sem_cmp_binarith'; auto);
+  try (destruct OP; subst op;
+  iIntros "(% & H & %)";
     repeat match goal with
-    |  H: app_pred (denote_tc_assert  (tc_andp' _ _) _) _ |- _ => 
-                                destruct H
-    | H:  app_pred   (denote_tc_assert
-          (check_pp_int' _ _ _ _ _) _) _ |- _ => unfold check_pp_int' in H
     | H: _ /\ _ |- _ => destruct H
-    | H: app_pred (denote_tc_assert (tc_bool _ _) _) _ |- _ => 
-                      apply tc_bool_e in H
     | H: negb (eqb_type ?A ?B) = true |- _ =>
              let J := fresh "J" in
               destruct (eqb_type A B) eqn:J; [inv H | clear H]
-    | H: app_pred (denote_tc_assert (tc_test_eq' _ _) _) _ |- _ =>
-           simpl in H; super_unfold_lift; simpl in H;
-            unfold Clight_Cop2.sem_cast, Clight_Cop2.classify_cast, size_t, sem_cast_pointer in H;
-            simpl in H; rewrite ?Hp in H; simpl in H
-   end;
-  unfold denote_tc_test_eq, sem_cast_i2l, sem_cast_l2l, cast_int_long, force_val in H1;
-  rewrite Hp in H1;
-
-    destruct (typeof e1) as [| [| | |] [|] | | | | | | |]; inv TV1; 
-    destruct (typeof e2) as [| [| | |] [|] | | | | | | |]; inv TV2;
-    simpl in H; inv H;
-    try (rewrite J in *; clear J);
-    try (rewrite J0 in *; clear J0);
-    destruct (eval_expr e1 rho), (eval_expr e2 rho);
-    try contradiction;
-    repeat match goal with
-    | H: app_pred (andp _ _) _ |- _ => destruct H
-    | H: app_pred (prop _) _ |- _ => do 3 red in H; subst
+    | |-context[denote_tc_test_eq _ _] =>
+           unfold Clight_Cop2.sem_cast, Clight_Cop2.classify_cast, size_t, sem_cast_pointer;
+           simpl; rewrite ?Hp; simpl
     end;
+  unfold denote_tc_test_eq, sem_cast_i2l, sem_cast_l2l, cast_int_long, force_val;
+  rewrite ?Hp; inv TV1; try (rewrite H in Hty1; try solve [destruct sz; inv Hty1]; try solve [destruct sz0; inv Hty1]; inv Hty1);
+  inv TV2; try (rewrite H3 in Hty2; try solve [destruct sz; inv Hty2]; try solve [destruct sz0; inv Hty2]; inv Hty2);
+  rewrite -> ?J, ?J0 in *;
+  destruct (eval_expr e1 rho); try contradiction; try iDestruct "H" as "[]";
+  destruct (eval_expr e2 rho); try iDestruct "H" as "[]"; try iDestruct "H" as "[-> ->]"; try iDestruct "H" as "[-> H]"; try done;
+    repeat match goal with
+    | H:  _ /\ _ |- _ => destruct H
+    end; subst;
     simpl; unfold Vptrofs, sem_cmp_pi, sem_cmp_ip, sem_cmp_pl, sem_cmp_lp, sem_cmp_pp; simpl; rewrite ?Hp; simpl;
     rewrite ?Hp; simpl;
-    try (rewrite (Ptrofs_to_of64_lemma Hp); 
-           unfold cast_int_int in H; rewrite H, Int.eq_true);
+    try (rewrite (Ptrofs_to_of64_lemma Hp);
+           unfold cast_int_int in H; rewrite Hii Int.eq_true);
     try (apply int_type_tc_val_Vtrue; auto);
     try (apply int_type_tc_val_Vfalse; auto);
     try (apply int_type_tc_val_of_bool; auto);
@@ -148,45 +136,14 @@ try abstract (
        change (Int64.eq (Ptrofs.to_int64 (Ptrofs.of_intu Int.zero)) Int64.zero) with true;
        simpl
     end;
-    try solve [if_tac; apply int_type_tc_val_of_bool; auto];
-   try solve [apply int_type_tc_val_Vfalse; auto];
-   try solve [apply int_type_tc_val_Vtrue; auto]).
+   try solve [iPureIntro; apply int_type_tc_val_of_bool; auto];
+   try solve [iPureIntro; if_tac; apply int_type_tc_val_of_bool; auto];
+   try solve [iPureIntro; apply int_type_tc_val_Vfalse; auto];
+   try solve [iPureIntro; apply int_type_tc_val_Vtrue; auto]);
+  match goal with |- context [match typeof e1 with _ => _ end] => destruct (typeof e1); try discriminate; try iDestruct "H" as "[]"
+                | |- context [match typeof e2 with _ => _ end] => destruct (typeof e2); try discriminate; try iDestruct "H" as "[]" end;
+  try iDestruct "H" as "[-> _]"; try (destruct s; iDestruct "H" as "[%Hs _]"; (apply Int64repr_Intsigned_zero in Hs as -> || apply Int64repr_Intunsigned_zero in Hs as ->); destruct si; simpl);
+  try solve [iPureIntro; apply int_type_tc_val_of_bool; auto].
+Qed.
 
-1,4:
- apply tc_bool_e in IBR;
- repeat rewrite andb_true_iff in IBR; destruct IBR as [[? ?] ?];
-    destruct (typeof e1) as [| [| | |] [|] | | | | | | |]; inv TV1; inv H0;
-    destruct (typeof e2) as [| [| | |] [|] | | | | | | |]; inv TV2; inv H1;
-    simpl in H; inv H;
-    destruct (eval_expr e1 rho), (eval_expr e2 rho);
-    try contradiction;
-   destruct OP; subst op; try destruct s; try destruct s0;
-  unfold sem_cmp_default, op_to_cmp,
- Clight_Cop2.sem_binarith, classify_binarith, both_int, both_long, Clight_Cop2.sem_cast,
-  Clight_Cop2.classify_cast, binarith_type; rewrite ?Hp;
-  simpl; rewrite ?Hp;
-    try (apply int_type_tc_val_Vtrue; auto);
-    try (apply int_type_tc_val_Vfalse; auto);
-    try (apply int_type_tc_val_of_bool; auto).
-
-all:
-destruct IBR as [IBR ?];
-apply tc_bool_e in IBR;
-rewrite negb_true_iff in IBR;
-unfold sem_cmp_pl, sem_cmp_lp, sem_cmp_pp, Val.cmplu_bool, Val.cmpu_bool;
-rewrite IBR, Hp;
-destruct (typeof e1) as [| [| | |] [|] | | | | | | |] eqn:He1;  inv TV1;
-destruct (typeof e2) as [| [| | |] [|] | | | | | | |] eqn:He2; inv TV2; inv H;
-try rewrite IBR in *;
-unfold check_pp_int' in H0;
-destruct OP; subst op; simpl; destruct H0 as [H0 H2]; apply tc_bool_e in H2;
-simpl in H0; unfold_lift in H0;
-unfold denote_tc_test_eq in H0;
-unfold Vptrofs; rewrite Hp;
-destruct (eval_expr e1 rho); try contradiction;
-destruct (eval_expr e2 rho); try contradiction;
-unfold size_t in H0; rewrite ?Hp,?He1,?He2 in H0; simpl in H0; destruct H0; subst; simpl;
-try solve [apply int_type_tc_val_of_bool; auto];
-rewrite Ptrofs_to_of64_lemma by assumption; rewrite  H; 
-apply int_type_tc_val_of_bool; auto.
-Time Qed.  (* 23.5 sec *)
+End mpred.
