veric/expr_lemmas2.v
@@ -1,7 +1,6 @@
-Require Import VST.msl.msl_standard.
 Require Import VST.veric.Clight_base.
-Require Import VST.veric.compcert_rmaps.
 Require Import VST.veric.Clight_lemmas.
+Require Import VST.veric.res_predicates.
 Require Import VST.veric.mpred.
 Require Import VST.veric.tycontext.
 Require Import VST.veric.expr.
@@ -13,62 +12,59 @@ Require Import VST.veric.seplog. (*For definition of tycontext*)
 Import Cop.
 Import Cop2.
 Import Clight_Cop2.
-Import compcert.lib.Maps.
 Import Ctypes.
 
-Lemma eval_lvalue_ptr : forall {CS: compspecs} rho m e (Delta: tycontext) te ve ge,
+Section mpred.
+
+Context `{!heapGS Σ}.
+
+Lemma eval_lvalue_ptr : forall {CS: compspecs} rho e (Delta: tycontext) te ve ge,
 mkEnviron ge ve te = rho ->
 typecheck_var_environ ve (var_types Delta) ->
 typecheck_glob_environ ge (glob_types Delta) ->
-denote_tc_assert (typecheck_lvalue Delta e) rho m ->
-exists base, exists ofs, eval_lvalue e rho  = Vptr base ofs.
+denote_tc_assert (typecheck_lvalue Delta e) rho ⊢
+⌜exists base, exists ofs, eval_lvalue e rho = Vptr base ofs⌝.
 Proof.
 intros.
-induction e; eauto;
-try now inversion H2.
-*
-simpl. unfold eval_var.
-simpl in H2.
-unfold get_var_type in H2.
+induction e; eauto; simpl.
+(*try now inversion H2.*)
+* unfold typecheck_lvalue.
+rewrite /get_var_type.
 subst rho; simpl ve_of; simpl ge_of.
-destruct_var_types i eqn:H4&?H; rewrite H4 in H2;
- [| destruct_glob_types i eqn:?H&?H; rewrite H6 in H2 ].
-+ apply tc_bool_e in H2.
+destruct_var_types i eqn:H4&?H; rewrite H4;
+ [| destruct_glob_types i eqn:H6&?H; rewrite H6 ].
++ rewrite tc_bool_e; iPureIntro.
   exists b, Ptrofs.zero.
-  rewrite H3, H2.
-  auto.
-+ apply tc_bool_e in H2.
+  simpl. by rewrite /eval_var H2 H.
++ rewrite tc_bool_e; iPureIntro.
   exists b, Ptrofs.zero.
-  rewrite H3, H5.
-  auto.
-+ inv H2.
+  simpl. by rewrite /eval_var H3 H2.
++ iIntros "[]".
 *
-simpl in H2.
-rewrite !denote_tc_assert_andp in H2.
-destruct H2 as [[? ?] ?].
-simpl in H4.
-simpl.
+unfold typecheck_lvalue; fold typecheck_expr.
+rewrite !denote_tc_assert_andp /=; unfold_lift.
+iIntros "[_ %H4]".
 destruct (eval_expr e rho); simpl; try now inversion H4; eauto.
 *
+unfold typecheck_lvalue; fold typecheck_lvalue.
+rewrite denote_tc_assert_andp.
 simpl in *. super_unfold_lift.
-rewrite denote_tc_assert_andp in H2.
-destruct H2.
-spec IHe; auto. destruct IHe.
+rewrite IHe; iIntros "[%IH H]".
 unfold eval_field.
-destruct H4 as [ofs ?].
+destruct IH as (base & ofs & IH).
 destruct (eval_lvalue e rho); try congruence.
-inversion H4; subst x i0; clear H4.
-destruct (typeof e); try now inversion H3.
+inv IH.
+destruct (typeof e); try iDestruct "H" as "[]".
 +
-destruct (cenv_cs ! i0) as [co |]; [| inv H3].
-destruct (field_offset cenv_cs i (co_members co)); [| inv H3].
-destruct p. destruct b0; [ | inv H3].
+destruct (cenv_cs !! i0) as [co |]; [| iDestruct "H" as "[]"].
+destruct (field_offset cenv_cs i (co_members co)); [| iDestruct "H" as "[]"].
+destruct p. destruct b; [ | iDestruct "H" as "[]"].
 unfold offset_val; eauto.
 +
-destruct (cenv_cs ! i0) as [co |]; [| inv H3].
-destruct (union_field_offset cenv_cs i (co_members co)); [| inv H3].
-destruct p. destruct z; [ | inv H3 .. ].
-destruct b0; [ | inv H3].
+destruct (cenv_cs !! i0) as [co |]; [| iDestruct "H" as "[]"].
+destruct (union_field_offset cenv_cs i (co_members co)); [| iDestruct "H" as "[]"].
+destruct p. destruct z; [ | iDestruct "H" as "[]" .. ].
+destruct b; [ | iDestruct "H" as "[]"].
 simpl.
 eauto.
 Qed.
@@ -84,35 +80,37 @@ unfold denote_tc_nodivover in *;
 unfold denote_tc_initialized in *.
 
 Lemma typecheck_lvalue_Evar:
-  forall {CS: compspecs} i t pt Delta rho m, typecheck_environ Delta rho ->
-           denote_tc_assert (typecheck_lvalue Delta (Evar i t)) rho m ->
-           is_pointer_type pt = true ->
-           tc_val pt (eval_lvalue (Evar i t) rho).
+  forall {CS: compspecs} i t pt Delta rho, typecheck_environ Delta rho ->
+           denote_tc_assert (typecheck_lvalue Delta (Evar i t)) rho ⊢
+           ⌜is_pointer_type pt = true ->
+            tc_val pt (eval_lvalue (Evar i t) rho)⌝.
 Proof.
 intros.
-simpl in *. unfold eval_var.
+unfold typecheck_lvalue.
+simpl. unfold eval_var.
 
 unfold typecheck_environ in H.
 intuition.
 destruct rho.
 unfold get_var_type in *.
 
-destruct_var_types i; rewrite ?Heqo, ?Heqo0 in *; try rewrite eqb_type_eq in *; simpl in *; intuition.
-remember (type_eq t t0). destruct s; try tauto.
+destruct_var_types i; rewrite -> ?Heqo, ?Heqo0 in *; try rewrite -> eqb_type_eq in *; simpl in *; intuition.
+rewrite tc_bool_e; iPureIntro; intros.
+remember (type_eq t t0). destruct s; try discriminate.
 {
 simpl in *.
- unfold is_pointer_type in H1.
- destruct pt; try solve [inv H1; auto].
+ unfold is_pointer_type in *.
+ destruct pt; try solve [inv H3; simpl in *; auto].
  unfold tc_val.
  simple_if_tac; apply I.
 }
-{destruct_glob_types i; rewrite ?Heqo1, ?Heqo2 in *; [| inv H0].
+{ destruct_glob_types i; rewrite -> ?Heqo1, ?Heqo2 in *; [| iIntros "[]"].
 remember (eqb_type t t0).
-symmetry in Heqb0. destruct b0; simpl in *; [| inv H0]. apply eqb_type_true in Heqb0.
+symmetry in Heqb0. destruct b0; simpl in *; [| iIntros "[]"]. apply eqb_type_true in Heqb0.
 subst.
-
-unfold tc_val; unfold is_pointer_type in H1;
- destruct pt; try solve [inv H1; reflexivity].
+iPureIntro; intros.
+unfold tc_val; unfold is_pointer_type in H3;
+ destruct pt; try solve [inv H3; reflexivity].
  simple_if_tac; apply I.
 }
 Qed.
@@ -128,111 +126,120 @@ Proof.
 Qed.
 
 Lemma typecheck_expr_sound_Efield:
-  forall {CS: compspecs} Delta rho e i t m
+  forall {CS: compspecs} Delta rho e i t
   (H: typecheck_environ Delta rho)
-  (IHe: (denote_tc_assert (typecheck_expr Delta e) rho m ->
-          tc_val (typeof e) (eval_expr e rho)) /\
+  (IHe: (denote_tc_assert (typecheck_expr Delta e) rho ⊢
+          ⌜tc_val (typeof e) (eval_expr e rho)⌝) /\
           (forall pt : type,
-          denote_tc_assert (typecheck_lvalue Delta e) rho m ->
-          is_pointer_type pt = true ->
-          tc_val pt (eval_lvalue e rho)))
-  (H0: denote_tc_assert (typecheck_expr Delta (Efield e i t)) rho m),
-  tc_val (typeof (Efield e i t)) (eval_expr (Efield e i t) rho).
+          denote_tc_assert (typecheck_lvalue Delta e) rho ⊢
+          ⌜is_pointer_type pt = true ->
+          tc_val pt (eval_lvalue e rho)⌝)),
+  denote_tc_assert (typecheck_expr Delta (Efield e i t)) rho ⊢
+  ⌜tc_val (typeof (Efield e i t)) (eval_expr (Efield e i t) rho)⌝.
 Proof.
 intros.
-simpl in *. super_unfold_lift.
+simpl in *. unfold typecheck_expr; fold typecheck_lvalue. super_unfold_lift.
  unfold eval_field, offset_val, deref_noload in *.
-assert (MODE: access_mode t = By_reference) by (destruct (access_mode t); auto; hnf in H0; try contradiction).
-rewrite MODE in *.
-destruct IHe.
+iIntros "H".
+iAssert (⌜access_mode t = By_reference⌝)%I with "[H]" as %MODE. by (destruct (access_mode t); auto; hnf in H0; try contradiction).
+rewrite MODE.
+destruct IHe as [IHe IHl].
 destruct rho.
-rewrite denote_tc_assert_andp in H0. destruct H0.
+rewrite denote_tc_assert_andp.
 unfold typecheck_environ in H.
 destruct H as [_ [Hve Hge]].
-assert (PTR := eval_lvalue_ptr _ _ e Delta te ve ge (eq_refl _) Hve Hge H0).
-specialize (H2 t H0).
-spec H2. clear - MODE; destruct t; try destruct i; try destruct s; try destruct f; inv MODE; simpl; auto.
-destruct PTR.
-destruct (typeof e); try now inv H3.
-+ destruct (cenv_cs ! i0) as [co |]; try now inv H3.
-  destruct (field_offset cenv_cs i (co_members co)) as [ [ ? [|]] |  ]; try now inv H3.
+iDestruct (eval_lvalue_ptr with "[H]") as %PTR; first done.
+{ by rewrite bi.and_elim_l. }
+rewrite (IHl t); iDestruct "H" as (He) "H".
+spec He. { clear - MODE; destruct t; try destruct i; try destruct s; try destruct f; inv MODE; simpl; auto. }
+destruct PTR as (? & ? & H); simpl in H.
+destruct (typeof e); try iDestruct "H" as "[]".
++ destruct (cenv_cs !! i0) as [co |]; try iDestruct "H" as "[]".
+  destruct (field_offset cenv_cs i (co_members co)) as [ [ ? [|]] |  ]; try iDestruct "H" as "[]".
   destruct (eval_lvalue e (mkEnviron ge ve te)); try now inv H.
-  destruct t; auto; try inversion H2.
-  destruct f; inv H2.
-  red. simple_if_tac; apply I.
-+ destruct (cenv_cs ! i0) as [co |]; try now inv H3.
-  destruct (union_field_offset cenv_cs i (co_members co)) as [ [ ? [|]] |  ]; try contradiction;
-  destruct z; try contradiction.
+  destruct t; auto; inv H.
+  destruct f; inv He.
++ destruct (cenv_cs !! i0) as [co |]; try iDestruct "H" as "[]".
+  destruct (union_field_offset cenv_cs i (co_members co)) as [ [ ? [|]] |  ]; try iDestruct "H" as "[]";
+  destruct z; try iDestruct "H" as "[]".
   destruct (eval_lvalue e (mkEnviron ge ve te)); try now inv H.
   rewrite ptrofs_add_repr_0; auto.
 Qed.
 
 Lemma typecheck_lvalue_sound_Efield:
- forall {CS: compspecs} Delta rho m e i t pt
+ forall {CS: compspecs} Delta rho e i t pt
  (H: typecheck_environ Delta rho)
- (IHe: (denote_tc_assert (typecheck_expr Delta e) rho m ->
-          tc_val (typeof e) (eval_expr e rho)) /\
-        (forall pt0 : type, denote_tc_assert (typecheck_lvalue Delta e) rho m ->
-           is_pointer_type pt0 = true ->
-         tc_val pt0 (eval_lvalue e rho)))
-  (H0: denote_tc_assert (typecheck_lvalue Delta (Efield e i t)) rho m)
+ (IHe: (denote_tc_assert (typecheck_expr Delta e) rho ⊢
+          ⌜tc_val (typeof e) (eval_expr e rho)⌝) /\
+        (forall pt0 : type, denote_tc_assert (typecheck_lvalue Delta e) rho ⊢
+           ⌜is_pointer_type pt0 = true ->
+         tc_val pt0 (eval_lvalue e rho)⌝))
   (H1: is_pointer_type pt = true),
-  tc_val pt (eval_lvalue (Efield e i t) rho).
+  denote_tc_assert (typecheck_lvalue Delta (Efield e i t)) rho ⊢
+  ⌜tc_val pt (eval_lvalue (Efield e i t) rho)⌝.
 Proof.
 intros.
 simpl in *.
-rewrite denote_tc_assert_andp in H0. destruct H0.
+unfold typecheck_lvalue; fold typecheck_lvalue.
+rewrite denote_tc_assert_andp.
 super_unfold_lift.
+destruct IHe as [IHe IHl].
  unfold eval_field,offset_val in *; intuition.
-specialize  (H4 pt).
 destruct rho.
 unfold typecheck_environ in *. intuition.
-assert (PTR := eval_lvalue_ptr _ m e _ te _ _ (eq_refl _) H H7 H0).
-simpl in *.
+iIntros "H".
+iDestruct (eval_lvalue_ptr with "[H]") as %PTR; first done.
+{ by rewrite bi.and_elim_l. }
+rewrite (IHl pt); iDestruct "H" as (Hpt) "H".
+spec Hpt; first done.
 remember (eval_lvalue e (mkEnviron ge ve te)). unfold isptr in *.
 subst v.
 destruct PTR as [b [ofs ?]].
-destruct (typeof e); try now inv H2.
-+ destruct (cenv_cs ! i0) as [co |]; try now inv H2.
-  destruct (field_offset cenv_cs i (co_members co)) as [ [ ? [|]] |  ]; try now inv H2.
-  destruct (eval_lvalue e (mkEnviron ge ve te)); try now inv H6.
-  destruct pt; inv H1; auto.
+destruct (typeof e); try iDestruct "H" as "[]".
++ destruct (cenv_cs !! i0) as [co |]; try iDestruct "H" as "[]".
+  destruct (field_offset cenv_cs i (co_members co)) as [ [ ? [|]] |  ]; try iDestruct "H" as "[]".
+  iPureIntro; intros.
+  rewrite H2.
+  destruct pt; inv H1; simpl; auto.
   red; simple_if_tac; apply I.
-+ destruct (cenv_cs ! i0) as [co |]; try now inv H2.
-  destruct (union_field_offset cenv_cs i (co_members co)) as [ [ ? [|]] |  ]; try now inv H2.
-  2: destruct z; contradiction.
-  destruct z; try contradiction.
-  destruct (eval_lvalue e (mkEnviron ge ve te)); try now inv H6.
++ destruct (cenv_cs !! i0) as [co |]; try iDestruct "H" as "[]".
+  destruct (union_field_offset cenv_cs i (co_members co)) as [ [ ? [|]] |  ]; try iDestruct "H" as "[]".
+  2: destruct z; iDestruct "H" as "[]".
+  destruct z; try iDestruct "H" as "[]".
+  iPureIntro; intros.
+  rewrite H2 in Hpt |- *.
   rewrite ptrofs_add_repr_0; auto.
 Qed.
 
 Lemma typecheck_expr_sound_Evar:
-  forall {CS: compspecs} Delta rho m i t,
+  forall {CS: compspecs} Delta rho i t,
   typecheck_environ Delta rho ->
-  denote_tc_assert (typecheck_expr Delta (Evar i t)) rho m ->
-  tc_val (typeof (Evar i t)) (eval_expr (Evar i t) rho).
+  denote_tc_assert (typecheck_expr Delta (Evar i t)) rho ⊢
+  ⌜tc_val (typeof (Evar i t)) (eval_expr (Evar i t) rho)⌝.
 Proof.
 intros.
-assert (MODE: access_mode t = By_reference)
- by (unfold typecheck_expr in H0; destruct (access_mode t); try (hnf in H0; contradiction); auto).
-simpl. super_unfold_lift. unfold deref_noload.
+unfold typecheck_expr.
+iIntros "H".
+iAssert (⌜access_mode t = By_reference⌝)%I with "[H]" as %MODE. by (destruct (access_mode t); auto; try contradiction).
+rewrite MODE.
+simpl.
 
 unfold typecheck_environ in H. intuition.
 destruct rho.
-simpl in H0. rewrite MODE in H0.
 unfold get_var_type in *.
 
 unfold eval_var.
-destruct_var_types i; rewrite ?Heqo, ?Heqo0 in *;
-try rewrite eqb_type_eq in *; simpl in *; intuition.
-- remember (type_eq t t0). destruct s; try tauto.
+destruct_var_types i; rewrite -> ?Heqo, ?Heqo0 in *;
+try rewrite -> eqb_type_eq in *; simpl in *; intuition.
+- rewrite tc_bool_e; iDestruct "H" as %?; iPureIntro.
+remember (type_eq t t0). destruct s; try discriminate.
  subst.
  simpl.
-simpl. destruct t0; try destruct i0; try destruct s; try destruct f; inv MODE; simpl; auto.
-- destruct_glob_types i; rewrite ?Heqo1, ?Heqo2 in *; [| inv H0].
-simpl in *.
+destruct t0; try destruct i0; try destruct s; try destruct f; inv MODE; simpl; auto.
+- destruct_glob_types i; rewrite -> ?Heqo1, ?Heqo2 in *; [| iDestruct "H" as "[]"].
+rewrite tc_bool_e; iDestruct "H" as %?; iPureIntro.
 remember (eqb_type t t0).
-symmetry in Heqb0. destruct b0; simpl in *; [| inv H0].
+symmetry in Heqb0. destruct b0; simpl in *; [| done].
 apply eqb_type_true in Heqb0.
 subst.
 unfold typecheck_glob_environ in *.
@@ -265,14 +272,6 @@ match op with
 end.
 
 
-Lemma tc_bool_e: forall {CS: compspecs} b a rho m, (* copied from binop_lemmas.v *)
-  app_pred (denote_tc_assert (tc_bool b a) rho) m ->
-  b = true.
-Proof.
-intros.
-destruct b; simpl in H; auto.
-Qed.
-
 Lemma tc_val_of_bool_int_type:
  forall b t, is_int_type t = true ->
   tc_val t (bool2val b).
@@ -284,50 +283,45 @@ rewrite <- Z.leb_le; reflexivity.
 Qed.
 
 Lemma typecheck_unop_sound:
- forall {CS: compspecs} Delta rho m u e t
+ forall {CS: compspecs} Delta rho u e t
  (H: typecheck_environ Delta rho)
- (IHe: (denote_tc_assert (typecheck_expr Delta e) rho m ->
-          tc_val (typeof e) (eval_expr e rho)) /\
+ (IHe: (denote_tc_assert (typecheck_expr Delta e) rho ⊢
+          ⌜tc_val (typeof e) (eval_expr e rho)⌝) /\
           (forall pt : type,
-           denote_tc_assert (typecheck_lvalue Delta e) rho m ->
-           is_pointer_type pt = true ->
-           tc_val pt (eval_lvalue e rho)))
-  (H0: denote_tc_assert (typecheck_expr Delta (Eunop u e t)) rho m),
-  tc_val t (eval_expr (Eunop u e t) rho).
+           denote_tc_assert (typecheck_lvalue Delta e) rho ⊢
+           ⌜is_pointer_type pt = true ->
+           tc_val pt (eval_lvalue e rho)⌝)),
+  denote_tc_assert (typecheck_expr Delta (Eunop u e t)) rho ⊢
+  ⌜tc_val t (eval_expr (Eunop u e t) rho)⌝.
 Proof.
 intros.
-simpl in H0. rewrite denote_tc_assert_andp in H0. destruct H0.
-destruct IHe as [? _].
-specialize (H2 H1).
-simpl eval_expr.
+unfold typecheck_expr; fold typecheck_expr.
+rewrite denote_tc_assert_andp /=.
+destruct IHe as [IHe _].
+rewrite IHe. iIntros "[H %H2]".
 unfold_lift.
-clear - H2 H0. 
+clear IHe.
 unfold eval_unop, sem_unary_operation, force_val1.
-destruct u; unfold tc_val in H2; simpl in H0;
-unfold sem_notbool, sem_notint, sem_neg, sem_absfloat, bool_val in *;
-super_unfold_lift; simpl;
+Local Opaque eqb_type.
+destruct u; unfold tc_val in H2; simpl;
+unfold sem_notbool, sem_notint, sem_neg, sem_absfloat, bool_val;
 destruct (typeof e) as [ | [ | | | ] [ | ] | | [ | ] | | | | | ];
- try contradiction;
- repeat match goal with
- | H:  app_pred (denote_tc_assert (tc_andp _ _) _) _ |- _ =>
-        rewrite denote_tc_assert_andp in H; destruct H
- | H: app_pred (denote_tc_assert (tc_bool _ _) _) _ |- _ => 
-      apply tc_bool_e in H
- | H: app_pred (denote_tc_assert (tc_int_or_ptr_type _) _) _ |- _ => 
-      apply tc_bool_e in H
-| H: (if eqb_type ?T1 ?T2 then _ else _) _ |- _ =>
+ try done; rewrite ?denote_tc_assert_andp /= ?tc_bool_e; unfold_lift;
+(iDestruct "H" as "%" || (rewrite ?assoc; iDestruct "H" as "[% _]")); iPureIntro;
+    repeat match goal with
+    | H: _ /\ _ |- _ => destruct H
+    | H: (if eqb_type ?T1 ?T2 then _ else _) _ |- _ =>
    let J := fresh "J" in
    destruct (eqb_type T1 T2) eqn:J;
    [apply eqb_type_true in J | apply eqb_type_false in J]
 end;
- destruct (eval_expr e rho) eqn:?; try contradiction;
- try discriminate;
+ destruct (eval_expr e rho) eqn:?; try done;
  try solve [apply tc_val_of_bool_int_type; auto].
 all: try solve [
   destruct t as [ | [ | | | ] [ | ] | | [ | ] | | | | | ]; 
   match goal with H: _ _ = true |- _ => inv H end;
             try reflexivity; auto;
-             simpl tc_val; try split; auto;
+             unfold tc_val; try split; auto;
              rewrite <- Z.leb_le; reflexivity].
 Qed.
 
@@ -355,13 +349,13 @@ intros. destruct t1; destruct t2;
 Qed.
 
 Lemma typecheck_temp_sound:
-  forall {CS: compspecs} Delta rho m i t,
+  forall {CS: compspecs} Delta rho i t,
   typecheck_environ Delta rho ->
-  denote_tc_assert (typecheck_expr Delta (Etempvar i t)) rho m ->
-  tc_val (typeof (Etempvar i t)) (eval_expr (Etempvar i t) rho).
+  denote_tc_assert (typecheck_expr Delta (Etempvar i t)) rho ⊢
+  ⌜tc_val (typeof (Etempvar i t)) (eval_expr (Etempvar i t) rho)⌝.
 Proof.
 intros.
-simpl in *. destruct rho.
+simpl. unfold typecheck_expr. destruct rho.
 destruct H as [H1 _].
 unfold typecheck_temp_environ in *.
 unfold eval_id, force_val in *.
@@ -370,19 +364,21 @@ simpl.
 destruct Delta; simpl in *.
 unfold temp_types in *. simpl in *.
 specialize (H1 i).
-destruct (tyc_temps ! i); try (contradiction H0).
-destruct (H1 _ (eq_refl _)) as [v ?]. clear H1.
-destruct H.
+destruct (tyc_temps !! i) eqn: Hty; try (iIntros "[]").
+destruct (H1 _ Hty) as (v & H & Ht0). clear H1.
 rewrite H.
-simpl in H0.
 destruct (is_neutral_cast t0 t) eqn:?.
-+ simpl in H0.
++ simpl.
+  unfold denote_tc_initialized.
+  iPureIntro; intros H0.
   rewrite H in H0.
   destruct H0 as [? [? ?]].
   inv H0.
   symmetry in Heqb; eapply neutral_cast_subsumption; eauto.
-+ destruct (same_base_type t0 t) eqn:?; [ | inv H0].
-  simpl in H0.
++ destruct (same_base_type t0 t) eqn:?; [ | iIntros "[]"].
+  simpl.
+  unfold denote_tc_initialized.
+  iPureIntro; intros H0.
   rewrite H in H0.
   destruct H0 as [? [? ?]].
   inv H0.
@@ -390,33 +386,30 @@ destruct (is_neutral_cast t0 t) eqn:?.
 Qed.
 
 Lemma typecheck_deref_sound:
-  forall {CS: compspecs} Delta rho m e t pt,
+  forall {CS: compspecs} Delta rho e t pt,
    typecheck_environ Delta rho ->
-   (denote_tc_assert (typecheck_expr Delta e) rho m ->
-    tc_val (typeof e) (eval_expr e rho)) /\
+   (denote_tc_assert (typecheck_expr Delta e) rho ⊢
+    ⌜tc_val (typeof e) (eval_expr e rho)⌝) /\
     (forall pt0 : type,
-     denote_tc_assert (typecheck_lvalue Delta e) rho m ->
-     is_pointer_type pt0 = true -> tc_val pt0 (eval_lvalue e rho)) ->
-     denote_tc_assert (typecheck_lvalue Delta (Ederef e t)) rho m ->
-    is_pointer_type pt = true ->
-    tc_val pt (eval_lvalue (Ederef e t) rho).
+     denote_tc_assert (typecheck_lvalue Delta e) rho ⊢
+     ⌜is_pointer_type pt0 = true -> tc_val pt0 (eval_lvalue e rho)⌝) ->
+     denote_tc_assert (typecheck_lvalue Delta (Ederef e t)) rho ⊢
+    ⌜is_pointer_type pt = true ->
+     tc_val pt (eval_lvalue (Ederef e t) rho)⌝.
 Proof.
-intros until pt. intros H IHe H0 H1.
-simpl. unfold lift.
-simpl in H0.
-repeat rewrite denote_tc_assert_andp in H0.
-destruct H0 as [[? ?] ?].
-destruct IHe as[ ? _].
-specialize (H4 H0).
-revert H2; case_eq (is_pointer_type (typeof e)); intros; hnf in H2; try contradiction.
-clear H H5 H4.
-hnf in H3. unfold_lift in H3; hnf in H3.
-unfold_lift.
+intros until pt. intros H IHe.
+unfold typecheck_lvalue; fold typecheck_expr.
+simpl.
+rewrite !denote_tc_assert_andp tc_bool_e.
+iIntros "[[H %] %]".
+destruct IHe as [-> _]; iPureIntro; intros.
+revert H0; case_eq (is_pointer_type (typeof e)); intros; hnf in H0; try discriminate.
 destruct (eval_expr e rho); try contradiction.
-destruct pt; try solve [inv H1; reflexivity].
+destruct pt; try solve [inv H2; reflexivity].
 unfold tc_val.
-unfold is_pointer_type in H1.
-destruct (eqb_type (Tpointer pt a) int_or_ptr_type); inv H1.
+unfold is_pointer_type in H2.
+destruct (eqb_type (Tpointer pt a) int_or_ptr_type); inv H2.
 apply I.
 Qed.
 
+End mpred.
