veric/semax.v
@@ -1,5 +1,5 @@
 Require Import VST.veric.juicy_base.
-Require Import VST.veric.juicy_mem VST.veric.juicy_mem_lemmas VST.veric.juicy_mem_ops.
+Require Import VST.veric.juicy_mem (*VST.veric.juicy_mem_lemmas VST.veric.juicy_mem_ops*).
 Require Import VST.veric.res_predicates.
 Require Import VST.veric.extend_tc.
 Require Import VST.veric.Clight_seplog.
@@ -13,8 +13,6 @@ Require Import VST.veric.juicy_extspec.
 Require Import VST.veric.tycontext.
 Require Import VST.veric.expr2.
 Require Import VST.veric.expr_lemmas.
-Require Import VST.veric.own.
-Require Import VST.veric.fupd.
 Import compcert.lib.Maps.
 
 Import Ctypes Clight_core.
